Migrate Backtracker.Refinement to ValidPos

correctness/RegexCorrectness/Backtracker/Refinement.lean
@@ -4,101 +4,98 @@ import RegexCorrectness.Strategy
 set_option autoImplicit false
 
 open Regex (NFA)
-open Regex.Data (BitMatrix BoundedIterator)
+open Regex.Data (BitMatrix BVPos)
 open Regex.Strategy (materializeUpdates)
-open String (Pos)
+open String (ValidPos)
 namespace Regex.Backtracker
 
-variable {nfa : NFA} {wf : nfa.WellFormed} {startIdx maxIdx bufferSize : Nat}
+variable {s : String} {nfa : NFA} {wf : nfa.WellFormed} {startPos : ValidPos s} {bufferSize : Nat}
 
-def StackEntry.materialize (entryH : StackEntry HistoryStrategy nfa startIdx maxIdx) : StackEntry (BufferStrategy bufferSize) nfa startIdx maxIdx :=
-  ⟨materializeUpdates bufferSize entryH.update, entryH.state, entryH.it⟩
+def StackEntry.materialize (entryH : StackEntry (HistoryStrategy s) nfa startPos) : StackEntry (BufferStrategy s bufferSize) nfa startPos :=
+  ⟨materializeUpdates bufferSize entryH.update, entryH.state, entryH.pos⟩
 
-def materializeStack (stackH : List (StackEntry HistoryStrategy nfa startIdx maxIdx)) : List (StackEntry (BufferStrategy bufferSize) nfa startIdx maxIdx) :=
+def materializeStack (stackH : List (StackEntry (HistoryStrategy s) nfa startPos)) : List (StackEntry (BufferStrategy s bufferSize) nfa startPos) :=
   stackH.map StackEntry.materialize
 
 @[simp]
-theorem materializeStack.nil : materializeStack [] = ([] : List (StackEntry (BufferStrategy bufferSize) nfa startIdx maxIdx)) := rfl
+theorem materializeStack.nil : materializeStack [] = ([] : List (StackEntry (BufferStrategy s bufferSize) nfa startPos)) := rfl
 
 @[simp]
 theorem materializeStack.cons {entryH stackH} :
-  materializeStack (entryH :: stackH) = (StackEntry.materialize entryH :: materializeStack stackH : List (StackEntry (BufferStrategy bufferSize) nfa startIdx maxIdx)) := rfl
+  materializeStack (entryH :: stackH) = (StackEntry.materialize entryH :: materializeStack stackH : List (StackEntry (BufferStrategy s bufferSize) nfa startPos)) := rfl
 
-def materializeResultAux (resultH : Option (List (Nat × Pos.Raw)) × BitMatrix nfa.nodes.size (maxIdx + 1 - startIdx)) : Option (Buffer bufferSize) × BitMatrix nfa.nodes.size (maxIdx + 1 - startIdx) :=
+def materializeResultAux (resultH : Option (List (Nat × ValidPos s)) × BitMatrix nfa.nodes.size (startPos.remainingBytes + 1)) : Option (Buffer s bufferSize) × BitMatrix nfa.nodes.size (startPos.remainingBytes + 1) :=
   ⟨resultH.1.map (materializeUpdates bufferSize), resultH.2⟩
 
-def materializeResult (resultH : Option (List (Nat × Pos.Raw))) : Option (Buffer bufferSize) :=
+def materializeResult (resultH : Option (List (Nat × ValidPos s))) : Option (Buffer s bufferSize) :=
   resultH.map (materializeUpdates bufferSize)
 
-theorem captureNextAux.pushNext.refines {nfa wf startIdx maxIdx bufferSize stackH stackB updateH updateB state it}
-  (refEntry : StackEntry.materialize ⟨updateH, state, it⟩ = ⟨updateB, state, it⟩) (refStack : materializeStack stackH = stackB) :
-  materializeStack (captureNextAux.pushNext HistoryStrategy nfa wf startIdx maxIdx stackH updateH state it) = captureNextAux.pushNext (BufferStrategy bufferSize) nfa wf startIdx maxIdx stackB updateB state it := by
-  cases stackH, updateH, state, it using captureNextAux.pushNext.fun_cases' HistoryStrategy nfa wf startIdx maxIdx with
-  | done stackH updateH state it hn => simp [pushNext.done hn, refStack]
-  | fail stackH updateH state it hn => simp [pushNext.fail hn, refStack]
-  | epsilon stackH updateH state it state' hn =>
+theorem captureNextAux.pushNext.refines {s nfa wf startPos bufferSize stackH stackB updateH updateB state pos}
+  (refEntry : StackEntry.materialize ⟨updateH, state, pos⟩ = ⟨updateB, state, pos⟩) (refStack : materializeStack stackH = stackB) :
+  materializeStack (captureNextAux.pushNext (HistoryStrategy s) nfa wf startPos stackH updateH state pos) = captureNextAux.pushNext (BufferStrategy s bufferSize) nfa wf startPos stackB updateB state pos := by
+  cases stackH, updateH, state, pos using captureNextAux.pushNext.fun_cases' (HistoryStrategy s) nfa wf startPos with
+  | done stackH updateH state pos hn => simp [pushNext.done hn, refStack]
+  | fail stackH updateH state pos hn => simp [pushNext.fail hn, refStack]
+  | epsilon stackH updateH state pos state' hn =>
     simp [StackEntry.materialize] at refEntry
     simp [pushNext.epsilon hn, StackEntry.materialize, refStack, refEntry]
-  | split stackH updateH state it state₁ state₂ hn =>
+  | split stackH updateH state pos state₁ state₂ hn =>
     simp [StackEntry.materialize] at refEntry
     simp [pushNext.split hn, StackEntry.materialize, refStack, refEntry]
-  | save stackH updateH state it offset state' hn =>
+  | save stackH updateH state pos offset state' hn =>
     simp [StackEntry.materialize] at refEntry
     simp [pushNext.save hn, StackEntry.materialize, refStack, refEntry]
-  | anchor_pos stackH updateH state it a state' hn ht =>
+  | anchor_pos stackH updateH state pos a state' hn ht =>
     simp [StackEntry.materialize] at refEntry
     simp [pushNext.anchor_pos hn ht, StackEntry.materialize, refStack, refEntry]
-  | anchor_neg stackH updateH state it a state' hn ht =>
+  | anchor_neg stackH updateH state pos a state' hn ht =>
     simp [pushNext.anchor_neg hn ht, refStack]
-  | char_pos stackH updateH state it c state' hn hnext hc =>
+  | char_pos stackH updateH state pos c state' hn hnext hc =>
     simp [StackEntry.materialize] at refEntry
     simp [pushNext.char_pos hn hnext hc, StackEntry.materialize, refStack, refEntry]
-  | char_neg stackH updateH state it c state' hn h =>
+  | char_neg stackH updateH state pos c state' hn h =>
     simp [pushNext.char_neg hn h, refStack]
-  | sparse_pos stackH updateH state it cs state' hn hnext hc =>
+  | sparse_pos stackH updateH state pos cs state' hn hnext hc =>
     simp [StackEntry.materialize] at refEntry
     simp [pushNext.sparse_pos hn hnext hc, StackEntry.materialize, refStack, refEntry]
-  | sparse_neg stackH updateH state it cs state' hn h =>
+  | sparse_neg stackH updateH state pos cs state' hn h =>
     simp [pushNext.sparse_neg hn h, refStack]
 
-theorem captureNextAux.refines (nfa wf startIdx maxIdx bufferSize visited) {stackH stackB} (refStack : materializeStack stackH = stackB) :
-  materializeResultAux (captureNextAux HistoryStrategy nfa wf startIdx maxIdx visited stackH) = captureNextAux (BufferStrategy bufferSize) nfa wf startIdx maxIdx visited stackB := by
-  induction visited, stackH using captureNextAux.induct' HistoryStrategy nfa wf startIdx maxIdx generalizing stackB with
+theorem captureNextAux.refines {s} (nfa wf startPos bufferSize visited) {stackH stackB} (refStack : materializeStack stackH = stackB) :
+  materializeResultAux (captureNextAux (HistoryStrategy s) nfa wf startPos visited stackH) = captureNextAux (BufferStrategy s bufferSize) nfa wf startPos visited stackB := by
+  induction visited, stackH using captureNextAux.induct' (HistoryStrategy s) nfa wf startPos generalizing stackB with
   | base visited =>
     simp at refStack
     simp [refStack, captureNextAux_base, materializeResultAux]
-  | visited visited update state' it stackH mem ih =>
+  | visited visited update state' pos stackH mem ih =>
     simp at refStack
     simpa [←refStack, StackEntry.materialize, captureNextAux_visited mem] using ih rfl
-  | done visited update state' it stackH mem hn =>
+  | done visited update state' pos stackH mem hn =>
     simp at refStack
     simp [←refStack, StackEntry.materialize, captureNextAux_done mem hn, materializeResultAux]
-  | next visited update state' it stackH mem hn ih =>
+  | next visited update state' pos stackH mem hn ih =>
     simp at refStack
     simp [←refStack, StackEntry.materialize, captureNextAux_next mem hn]
     exact ih (pushNext.refines rfl rfl)
 
-theorem captureNext.go.refines (nfa wf startIdx bufferSize bit visited) :
-  materializeResult (captureNext.go HistoryStrategy nfa wf startIdx maxIdx bit visited) = captureNext.go (BufferStrategy bufferSize) nfa wf startIdx maxIdx bit visited := by
-  induction bit, visited using captureNext.go.induct' HistoryStrategy nfa wf startIdx maxIdx with
-  | found bit visited updateH visitedH hauxH =>
-    have hauxB := captureNextAux.refines nfa wf startIdx maxIdx bufferSize visited rfl (stackB := materializeStack [⟨HistoryStrategy.empty, ⟨nfa.start, wf.start_lt⟩, bit⟩])
+theorem captureNext.go.refines {s} (nfa wf startPos bufferSize bvpos visited) :
+  materializeResult (captureNext.go (HistoryStrategy s) nfa wf startPos bvpos visited) = captureNext.go (BufferStrategy s bufferSize) nfa wf startPos bvpos visited := by
+  induction bvpos, visited using captureNext.go.induct' (HistoryStrategy s) nfa wf startPos with
+  | found bvpos visited updateH visitedH hauxH =>
+    have hauxB := captureNextAux.refines nfa wf startPos bufferSize visited rfl (stackB := materializeStack [⟨(HistoryStrategy s).empty, ⟨nfa.start, wf.start_lt⟩, bvpos⟩])
     simp [↓hauxH, materializeResultAux] at hauxB
     simp [captureNext.go_found hauxH, captureNext.go_found hauxB.symm, materializeResult]
-  | not_found_next bit visited visitedH hauxH hnext ih =>
-    have hauxB := captureNextAux.refines nfa wf startIdx maxIdx bufferSize visited rfl (stackB := materializeStack [⟨HistoryStrategy.empty, ⟨nfa.start, wf.start_lt⟩, bit⟩])
+  | not_found_next bvpos visited visitedH hauxH ne ih =>
+    have hauxB := captureNextAux.refines nfa wf startPos bufferSize visited rfl (stackB := materializeStack [⟨(HistoryStrategy s).empty, ⟨nfa.start, wf.start_lt⟩, bvpos⟩])
     simp [↓hauxH, materializeResultAux] at hauxB
-    simpa [captureNext.go_not_found_next hauxH hnext, captureNext.go_not_found_next hauxB.symm hnext] using ih
-  | not_found_end bit visited visitedH hauxH hnext =>
-    have hauxB := captureNextAux.refines nfa wf startIdx maxIdx bufferSize visited rfl (stackB := materializeStack [⟨HistoryStrategy.empty, ⟨nfa.start, wf.start_lt⟩, bit⟩])
+    simpa [captureNext.go_not_found_next hauxH ne, captureNext.go_not_found_next hauxB.symm ne] using ih
+  | not_found_end bvpos visited visitedH hauxH ne =>
+    have hauxB := captureNextAux.refines nfa wf startPos bufferSize visited rfl (stackB := materializeStack [⟨(HistoryStrategy s).empty, ⟨nfa.start, wf.start_lt⟩, bvpos⟩])
     simp [↓hauxH, materializeResultAux] at hauxB
-    simp [captureNext.go_not_found_end hauxH hnext, captureNext.go_not_found_end hauxB.symm hnext, materializeResult]
+    simp [captureNext.go_not_found_end hauxH ne, captureNext.go_not_found_end hauxB.symm ne, materializeResult]
 
-theorem captureNext.refines (nfa wf bufferSize it) :
-  materializeResult (captureNext HistoryStrategy nfa wf it) = captureNext (BufferStrategy bufferSize) nfa wf it := by
-  if le : it.pos ≤ it.toString.endPos then
-    simpa [captureNext_le le] using captureNext.go.refines nfa wf it.pos.byteIdx bufferSize ⟨it, Nat.le_refl _, le, rfl⟩ (BitMatrix.zero _ _)
-  else
-    simp [captureNext_not_le le, materializeResult]
+theorem captureNext.refines {s} (nfa wf bufferSize pos) :
+  materializeResult (captureNext (HistoryStrategy s) nfa wf pos) = captureNext (BufferStrategy s bufferSize) nfa wf pos := by
+  simpa [captureNext] using captureNext.go.refines nfa wf pos bufferSize (BVPos.start pos) (BitMatrix.zero _ _)
 
 end Regex.Backtracker
